WIP

examples/generic.lean
@@ -5,3 +5,17 @@ open Qq Lean
 def listToExpr {α : Type} [ToExpr α] : List α → Q(List $α)
   | []       => q([])
   | a :: as  => q($a :: $(listToExpr as))
+
+def force_nat : Nat → Nat
+  := id
+
+structure Foo where
+  n : Nat
+
+example (foo : Foo) : Q(Foo) :=
+  let x := 1
+  let y := 2
+  let z := 1 + 2
+  let bar := Foo.mk z
+  let _ := force_nat z
+  q($bar)
